TaplLean/STLC/Env.lean
@@ -1,0 +1,4 @@
+import Batteries.Data.AssocList
+open Lean
+
+abbrev Env (α : Type) := AssocList String α
