TaplLean/STLC/Internal.lean
@@ -1,0 +1,15 @@
+inductive Ty : Type where
+  | TBool
+  | TArrow : Ty → Ty → Ty
+
+infix:100 " T.-> " => Ty.TArrow
+
+inductive Term : Type where
+  | tru
+  | fls
+  | ite : Term → Term → Term → Term
+  | var : String → Term
+  | abs : String → Ty → Term
+  | app : Term → Term → Term
+
+inductive WellTyped : Term → Ty → Prop where
